StructuredEncryption/src/Paths.dfy
@@ -26,7 +26,7 @@ module StructuredEncryptionPaths {
   {
     // Return the Canonical Path for this part of an item in this table
     function method canonicalPath(table : GoodString)
-      : (ret : Bytes)
+      : (ret : CanonicalPath)
       requires 0 < |parts|
       ensures ret ==
           //= specification/structured-encryption/header.md#canoncial-path
@@ -40,17 +40,17 @@ module StructuredEncryptionPaths {
           //= specification/structured-encryption/header.md#canoncial-path
           //= type=implication
           //# This MUST be followed by the encoding for each Structured Data in the path, including the Terminal itself.
-        + CanonicalPath(parts)
+        + MakeCanonicalPath(parts)
     {
       var tableName := UTF8.Encode(table).value;
       var depth := UInt64ToSeq(|parts| as uint64);
-      var path := CanonicalPath(parts);
+      var path := MakeCanonicalPath(parts);
       tableName + depth + path
     }
   }
 
   function method SimpleCanon(table : GoodString, attr : GoodString)
-    : Bytes
+    : CanonicalPath
   {
     TerminalLocation([Map(attr)]).canonicalPath(table)
   }
@@ -78,13 +78,13 @@ module StructuredEncryptionPaths {
   }
 
   // get the Canonical Path for these Selectors
-  function method {:tailrecursion} CanonicalPath(src : SelectorList)
-   : Bytes
+  function method {:tailrecursion} MakeCanonicalPath(src : SelectorList)
+   : CanonicalPath
   {
     if |src| == 0 then
       []
     else
-      CanonicalPart(src[0]) + CanonicalPath(src[1..])
+      CanonicalPart(src[0]) + MakeCanonicalPath(src[1..])
   }
 
 // End code, begin lemmas. 
@@ -116,7 +116,7 @@ module StructuredEncryptionPaths {
 
   lemma OnePart(src : SelectorList)
     requires |src| == 1
-    ensures CanonicalPath(src) == CanonicalPart(src[0])
+    ensures MakeCanonicalPath(src) == CanonicalPart(src[0])
   {}
 
   lemma SubstrNE<T>(x : seq<T>, y : seq<T>, len : nat)
